Big.thy
@@ -1,0 +1,26 @@
+theory Big
+  imports Common
+begin
+
+datatype 'a state = 
+     Reverse "'a current" "'a stack" "'a list" nat
+   | Common "'a Common.state"
+
+fun toList :: "'a state \<Rightarrow> 'a list" where
+  "toList (Common common) = Common.toList common"
+| "toList (Reverse current _ _ _) = Current.toList current"
+
+fun tick :: "'a state \<Rightarrow> 'a state" where
+  "tick (Common state) = Common (Common.tick state)"
+| "tick (Reverse current big auxB count) = 
+     Reverse current (Stack.pop big) ((first big)#auxB) (count - 1)"
+
+fun push :: "'a \<Rightarrow> 'a state \<Rightarrow> 'a state" where
+  "push x (Common state) = Common (Common.push x state)"
+| "push x (Reverse current big auxB count) = Reverse (put x current) big auxB count"
+
+fun pop :: "'a state \<Rightarrow> 'a * 'a state" where
+  "pop (Common state) = (let (x, state) = Common.pop state in (x, Common state))"
+| "pop (Reverse current big auxB count) = (top current, Reverse (bottom current) big auxB count)"
+
+end
