Big_Proof.thy
@@ -1,0 +1,9 @@
+theory Big_Proof
+  imports Big Common_Proof
+begin
+
+lemma tick: "toList (tick state) = toList state"
+  apply(induction state)
+  by(auto simp: tick)
+
+end
