Common.thy
@@ -1,0 +1,42 @@
+theory Common
+  imports Current Idle
+begin
+
+datatype 'a state = 
+    Copy "'a current" "'a list" "'a list" nat
+  | Idle "'a current" "'a idle"
+
+fun toList :: "'a state \<Rightarrow> 'a list" where
+  "toList (Idle current idle) = Current.toList current"
+| "toList (Copy current old new _) = Current.toList current"
+
+fun normalize :: "'a state \<Rightarrow> 'a state" where
+  "normalize (Copy current old new moved) = (
+      case current of Current extra added _ remained \<Rightarrow> 
+      if moved = remained
+      then Idle current (idle.Idle (Stack extra new) (added + moved))
+      else Copy current old new moved
+  )"
+| "normalize state = state"
+
+fun tick :: "'a state \<Rightarrow> 'a state" where
+  "tick (Idle current idle) = Idle current idle"
+| "tick (Copy current aux new moved) = (
+    case current of Current _ _ _ remained \<Rightarrow>
+      if moved < remained
+      then normalize (Copy current (tl aux) ((hd aux)#new) (moved + 1))
+      else normalize (Copy current aux new moved)
+  )"
+
+fun push :: "'a \<Rightarrow> 'a state \<Rightarrow> 'a state" where
+  "push x (Idle current (idle.Idle stack stackSize)) = 
+      Idle current (idle.Idle (Stack.push x stack) (Suc stackSize))"
+| "push x (Copy current aux new moved) = Copy (put x current) aux new moved"
+
+fun pop :: "'a state \<Rightarrow> 'a * 'a state" where
+  "pop (Idle current (idle.Idle stack stackSize)) = 
+      (first stack, Idle current (idle.Idle (Stack.pop stack) (stackSize - 1)))"
+| "pop (Copy current aux new moved) = 
+      (top current, Copy (bottom current) aux new moved)"
+
+end
