Common_Proof.thy
@@ -1,0 +1,9 @@
+theory Common_Proof
+  imports Common
+begin
+
+lemma tick: "toList (tick common) = toList common"
+  apply(induction common)
+  by(auto split: current.splits)
+
+end
