Deque_Proof.thy
@@ -1,5 +1,5 @@
 theory Deque_Proof
-  imports Deque Stack_Proof
+  imports Deque Transformation_Proof
 begin
 
 locale Deque =
@@ -14,100 +14,29 @@ fixes isEmpty :: "'q \<Rightarrow> bool"
 fixes listLeft :: "'q \<Rightarrow> 'a list"
 fixes listRight :: "'q \<Rightarrow> 'a list"
 fixes invariant :: "'q \<Rightarrow> bool"
+
 assumes listLeft_empty:     "listLeft empty = []"
 assumes listRight_empty:    "listRight empty = []"
+
 assumes list_enqueueLeft:   "invariant q \<Longrightarrow> listLeft(enqueueLeft x q) = x # listLeft q"
 assumes list_enqueueRight:  "invariant q \<Longrightarrow> listRight(enqueueRight x q) = x # listRight q"
+
 assumes list_dequeueLeft:   "invariant q \<Longrightarrow> \<not> listLeft q = [] \<Longrightarrow> listLeft(dequeueLeft q) = tl(listLeft q)"
 assumes list_dequeueRight:  "invariant q \<Longrightarrow> \<not> listRight q = [] \<Longrightarrow> listRight(dequeueRight q) = tl(listRight q)"
+
 assumes list_firstLeft:     "invariant q \<Longrightarrow> \<not> listLeft q = [] \<Longrightarrow> firstLeft q = hd(listLeft q)"
 assumes list_firstRight:    "invariant q \<Longrightarrow> \<not> listRight q = [] \<Longrightarrow> firstRight q = hd(listRight q)"
+
 assumes listLeft_isEmpty:   "invariant q \<Longrightarrow> isEmpty q = (listLeft q = [])"
 assumes listRight_isEmpty:  "invariant q \<Longrightarrow> isEmpty q = (listRight q = [])"
+
 assumes invariant_empty:        "invariant empty"
+
 assumes invariant_enqueueLeft:  "invariant q \<Longrightarrow> invariant(enqueueLeft x q)"
 assumes invariant_enqueueRight: "invariant q \<Longrightarrow> invariant(enqueueRight x q)"
+
 assumes invariant_dequeueLeft:  "invariant q \<Longrightarrow> \<not> isEmpty q  \<Longrightarrow> invariant(dequeueLeft q)"
 assumes invariant_dequeueRight: "invariant q \<Longrightarrow> \<not> isEmpty q  \<Longrightarrow> invariant(dequeueRight q)"
-
-lemma head: "xs \<noteq> [] \<Longrightarrow> hd xs = hd (xs @ ys)"
-  apply (induction xs arbitrary: ys)
-  by auto
-
-
-lemma test: "\<lbrakk>leftLength = length ll + length lr; rightLength = length rl + length rr; 2 \<le> length ll + length lr;
-        State2.ticks x1d x2d = (Reverse x11 x12 x13 x14, Reverse1 x11a x12a x13a); State2.ticks x1c x2c = (x1d, x2d);
-        State2.ticks x1b x2b = (x1c, x2c); State2.ticks x1a x2a = (x1b, x2b); State2.ticks x1 x2 = (x1a, x2a);
-        State2.ticks
-         (Reverse (Current [] 0 (Stack (x # ll) lr) (length ll + length lr - (length rl + length rr))) (Stack (x # ll) lr) []
-           (length ll + length lr - (length rl + length rr)))
-         (Reverse1 (Current [] 0 (Stack rl rr) (Suc (2 * length rl + 2 * length rr))) (Stack rl rr) []) =
-        (x1, x2);
-        \<not> Suc (length ll + length lr) \<le> 3 * length rl + 3 * length rr\<rbrakk>
-       \<Longrightarrow> Current.toList x11 @ rev (Current.toList x11a) = x # ll @ lr @ rev rr @ rev rl"
-  sorry
-
-lemma test3: 
-  assumes "2 \<le> length x1 + length x2"  
-          "Suc (length x1 + length x2) \<le> 3 * rightLength"
-          "rightLength \<le> 2"
-        shows "Deque.invariant (swap (toSmallDeque x1 x2))"
-proof-
-  from assms have "rightLength = 0 \<or> rightLength = 1 \<or> rightLength = 2"
-    by auto
-  
-  then show ?thesis 
-  proof
-    assume "rightLength = 0"
-    with assms show ?thesis
-      by auto
-  next
-    assume "rightLength = 1 \<or> rightLength = 2"
-    then have "rightLength = 1 \<or> rightLength = 2" .
-    then show ?thesis
-    proof
-      assume "rightLength = 1"
-      with assms show ?thesis
-        apply(induction x1 x2 rule: toSmallDeque.induct)
-        by auto
-    next
-      assume "rightLength = 2"
-      with assms show ?thesis
-        apply(induction x1 x2 rule: toSmallDeque.induct)
-        apply auto
-      sorry
-    qed
-  qed
-qed
-
-lemma testing: " \<lbrakk>
-  State2.ticks left3 right3 = (left4, Reverse1 current' small' auxS'); 
-  State2.ticks left2 right2 = (left3, right3); 
-  State2.ticks left1 right1 = (left2, right2);
-  State2.ticks (Reverse currentl big auxB count) (Reverse1 (put x currentr) small auxS) = (left1, right1)
-\<rbrakk> \<Longrightarrow> 
-  Current.toList current' @ rev (bToList left4 False) = x # Current.toList currentr @ rev (Current.toList currentl)"
-  apply(induction current' arbitrary: x small' auxS' rule: Current.toList.induct )
-  apply auto
-  apply(induction currentr rule: Current.toList.induct)
-  apply auto
-  apply(induction currentl rule: Current.toList.induct)
-  apply auto
-  apply(induction left4)
-   apply auto
-   apply(induction left3)
-    apply auto
-   apply(induction right3)
-     apply auto    
-  apply(induction left2)
-    apply auto
-   apply(induction right2)
-      apply auto
-   apply(induction left1)
-    apply auto
-   apply(induction right1 arbitrary: big auxB count small auxS)
-  apply auto
-  sorry
 
 
 interpretation RealtimeDeque: Deque where
@@ -145,24 +74,11 @@ next
     then show ?case by auto
   next
     case (Idle left right)
-    then show ?case 
-    proof(induction left)
-      case (Idle leftValues leftLength)
-      then show ?case
-      proof(induction right)
-        case (Idle rightValues rightLength)
-        then show ?case 
-        proof(induction leftValues)
-          case (Stack ll lr)
-          then show ?case 
-          proof(induction rightValues)
-            case (Stack rl rr)
-            then show ?case 
-              (* apply(auto simp: Let_def split: prod.splits stateS.splits stateB.splits) *)
-              sorry
-          qed
-        qed
-      qed
+    then show ?case
+    proof(induction x "Idle left right" rule: enqueueLeft.induct)
+      case (5 x left leftLength right rightLength)
+      then show ?case 
+        by (auto simp: push Let_def all_ticks split: prod.splits)
     qed
   next
     case (Transforming t x)
@@ -170,80 +86,21 @@ next
     proof(induction t arbitrary: x)
       case (Left left right)
       then show ?case 
-      proof(induction left)
-        case (Reverse1 currentl small auxS)
-        then show ?case
-        proof(induction right)
-          case (Reverse currentr big auxB count)
-          then show ?case
-            apply(auto simp: Let_def split: prod.splits stateS.splits stateB.splits)
-            sorry
-        next
-          case (Common x)
-          then show ?case sorry
-        qed
-      next
-        case (Reverse2 x1 x2 x3a x4 x5)
-        then show ?case sorry
-      next
-        case (Common x)
-        then show ?case sorry
-      qed
+        apply(auto simp: Let_def split: prod.splits state_splits)
+        sorry
     next
-      case (Right x1 x2)
-      then show ?case sorry
+      case (Right left right)
+      then show ?case
+         apply(auto simp: Let_def split: prod.splits state_splits)
+        sorry
     qed
   qed
 next
 case (4 q x)
-  then show ?case
-    sorry
+  then show ?case  sorry
 next
   case (5 q)
-  then show ?case
-  proof(induction q)
-  case Empty
-    then show ?case by auto
-  next
-    case (One x)
-    then show ?case by auto
-  next
-    case (Two x1 x2a)
-    then show ?case by auto
-  next
-    case (Three x1 x2a x3)
-    then show ?case by auto
-  next
-    case (Idle left right)
-    then show ?case
-    proof(induction left)
-      case (Idle stackl l)
-      then show ?case
-      proof(induction right)
-        case (Idle stackr r)
-        then show ?case 
-        proof(induction stackl arbitrary: l)
-          case (Stack ll lr)
-          then show ?case
-          proof(induction stackr arbitrary: r)
-            case (Stack rl rr)
-            then show ?case
-              apply(cases ll; cases lr; cases rl; cases rr)
-              subgoal 
-                by auto
-              subgoal
-                apply auto
-                sorry
-       
-              sorry 
-          qed
-        qed
-      qed
-    qed
-  next
-    case (Transforming x)
-    then show ?case sorry
-  qed 
+  then show ?case sorry
 next
   case (6 q)
   then show ?case sorry
@@ -273,40 +130,7 @@ next
   then show ?case sorry
 next
   case (15 q)
-  then show ?case
-  proof(induction q)
-    case Empty
-    then show ?case by auto
-    next
-    case (One x)
-    then show ?case by auto
-    next
-      case (Two x1 x2a)
-      then show ?case by auto
-    next
-      case (Three x1 x2a x3)
-      then show ?case by auto
-    next
-      case (Idle left right)
-      then show ?case 
-      proof(induction left)
-        case (Idle leftValues leftLength)
-        then show ?case
-        proof(induction right)
-          case (Idle rightValues rightLength)
-          then show ?case
-            apply(auto simp: Let_def pop size_pop not_empty)
-                   apply(auto simp: test3 split: prod.splits stack.splits)
-            sorry
-        qed
-      qed
-    next
-      case (Transforming x)
-      then show ?case sorry
-    qed
-  qed
-
-   
-
+  then show ?case sorry
+qed
 
 end
