Idle.thy
@@ -1,0 +1,10 @@
+theory Idle
+  imports Stack
+begin
+
+datatype 'a idle = Idle "'a stack" nat
+
+fun toList :: "'a idle \<Rightarrow> 'a list" where
+  "toList (Idle stack _) = Stack.toList stack"
+
+end
