Small.thy
@@ -1,0 +1,45 @@
+theory Small
+  imports Common
+begin
+
+datatype 'a state =
+   Reverse1 "'a current" "'a stack" "'a list"
+ | Reverse2 "'a current" "'a list" "'a stack" "'a list" nat
+ | Common "'a Common.state"
+
+fun toList :: "'a state \<Rightarrow> 'a list" where
+  "toList (Common common) = Common.toList common"
+| "toList (Reverse1 current _ _ ) = Current.toList current"
+| "toList (Reverse2 current _ _ _ _) = Current.toList current"
+
+fun tick :: "'a state \<Rightarrow> 'a state" where
+  "tick (Common state) = Common (Common.tick state)"
+| "tick (Reverse1 current small auxS) = (
+    if isEmpty small 
+    then Reverse1 current small auxS 
+    else Reverse1 current (Stack.pop small) ((first small)#auxS)
+  )"
+| "tick (Reverse2 current auxS big newS count) = (
+    if isEmpty big
+    then Common (normalize (Copy current auxS newS count))
+    else Reverse2 current auxS (Stack.pop big) ((first big)#newS) (count + 1)
+  )"
+
+
+
+fun push :: "'a \<Rightarrow> 'a state \<Rightarrow> 'a state" where
+  "push x (Common state) = Common (Common.push x state)"
+| "push x (Reverse1 current small auxS) = Reverse1 (put x current) small auxS"
+| "push x (Reverse2 current auxS big newS count) = Reverse2 (put x current) auxS big newS count"
+
+fun pop :: "'a state \<Rightarrow> 'a * 'a state" where
+  "pop (Common state) = (
+    let (x, state) = Common.pop state 
+    in (x, Common state)
+  )"
+| "pop (Reverse1 current small auxS) = 
+    (top current, Reverse1 (bottom current) small auxS)"
+| "pop (Reverse2 current auxS big newS count) = 
+    (top current, Reverse2 (bottom current) auxS big newS count)"
+
+end
