Transformation.thy
@@ -1,0 +1,33 @@
+theory Transformation 
+  imports Big Small
+begin
+
+fun ticksHelper :: "'a Big.state \<Rightarrow> 'a Small.state \<Rightarrow> 'a Big.state * 'a Small.state" where
+  "ticksHelper (Reverse currentB big auxB 0) (Reverse1 currentS _ auxS) =
+    (Big.Common (normalize (Copy currentB auxB [] 0)), Reverse2 currentS auxS big [] 0)"
+| "ticksHelper left right = (Big.tick left, Small.tick right)"
+
+datatype 'a transformation =
+   Left "'a Small.state" "'a Big.state"
+ | Right "'a Big.state" "'a Small.state"
+
+fun toListLeft :: "'a transformation \<Rightarrow> 'a list" where
+  "toListLeft (Left small big)  = Small.toList small  @ (rev (Big.toList big))"
+| "toListLeft (Right big small) = Big.toList big @ (rev (Small.toList small))"
+ 
+fun toListRight :: "'a transformation \<Rightarrow> 'a list" where
+  "toListRight (Left small big)  = Big.toList big @ (rev (Small.toList small))"
+| "toListRight (Right big small) = Small.toList small @ (rev (Big.toList big))"
+
+fun ticks :: "'a transformation \<Rightarrow> 'a transformation" where
+  "ticks (Left small big) = (case ticksHelper big small of (big, small) \<Rightarrow> Left small big)"
+| "ticks (Right big small) = (case ticksHelper big small of (big, small) \<Rightarrow> Right big small)"  
+
+fun fourTicks where
+  "fourTicks transformation = (ticks (ticks (ticks (ticks transformation))))"
+
+fun sixTicks where
+  "sixTicks transformation = ticks (ticks (fourTicks transformation))"
+
+
+end
