Transformation_Proof.thy
@@ -1,0 +1,59 @@
+theory Transformation_Proof
+  imports Transformation Small_Proof Big_Proof Stack_Proof
+begin
+
+lemmas tick = Small_Proof.tick Big_Proof.tick Common_Proof.tick
+
+lemma ticks: "toListLeft (ticks transformation) = toListLeft transformation"
+proof(induction transformation rule: toListLeft.induct)
+  case (1 small big)
+  
+  have "\<And>x1 x2. 
+        ticksHelper big small = (x1, x2) \<Longrightarrow>
+        Small.toList small @ rev (Big.toList big) = Small.toList x2 @ rev (Big.toList x1)"
+    apply(induction big small rule: ticksHelper.induct)
+    by(auto simp: tick split: current.splits)
+
+  then show ?case by (auto split: prod.splits)
+next
+  case (2 big small)
+
+  have "\<And>x1 x2. 
+        ticksHelper big small = (x1, x2) \<Longrightarrow>
+        Big.toList big @ rev (Small.toList small) = Big.toList x1 @ rev (Small.toList x2)"
+    apply(induction big small rule: ticksHelper.induct)
+    by(auto simp: tick split: current.splits)
+
+  then show ?case
+    by(auto split: prod.splits)
+qed
+
+lemma ticks_helper: "\<lbrakk>
+  ticksHelper
+         (Reverse (Current [] 0 (Stack.push x leftValues) (Stack.size leftValues - Stack.size rightValues)) (Stack.push x leftValues) [] (Stack.size leftValues - Stack.size rightValues))
+         (Reverse1 (Current [] 0 rightValues (Suc (2 * Stack.size rightValues))) rightValues []) = (left, right)
+    \<rbrakk>
+       \<Longrightarrow> Big.toList left @ rev (Small.toList right) = x # Stack.toList leftValues @ rev (Stack.toList rightValues)"
+proof(induction  
+         "Reverse (Current [] 0 (Stack.push x leftValues) (Stack.size leftValues - Stack.size rightValues)) (Stack.push x leftValues) [] (Stack.size leftValues - Stack.size rightValues)"
+         "Reverse1 (Current [] 0 rightValues (Suc (2 * Stack.size rightValues))) rightValues []"
+        rule: ticksHelper.induct
+        )
+  case 1
+  then show ?case 
+    by(auto simp: push)
+next
+  case ("2_1" vd)
+   then have left: "left = Big.tick (Reverse (Current [] 0 (Stack.push x leftValues) (Stack.size leftValues - Stack.size rightValues)) (Stack.push x leftValues) [] (Stack.size leftValues - Stack.size rightValues))"
+     by (metis ticksHelper.simps(2) prod.inject)
+   then have right: "right = Small.tick (Reverse1 (Current [] 0 rightValues (Suc (2 * Stack.size rightValues))) rightValues [])"
+     by (metis "2_1.hyps" "2_1.prems" ticksHelper.simps(2) old.prod.inject)
+   from left right show ?case
+     by(auto simp: push split: if_splits)
+ qed
+
+lemmas all_ticks = tick ticks ticks_helper
+
+lemmas state_splits = idle.splits Common.state.splits Small.state.splits Big.state.splits 
+
+end
